#### 9. 2)
a<sub>n</sub> = (n + 1)/(2n + 1) 
ε = 10<sup>-2</sup> 
|a<sub>n</sub> - A| < ε, A ∈ R 

A = 0 
|a<sub>n</sub> - A| < ε 
|(n + 1)/(2n + 1) - 0| < ε 
|(n + 1)/(2n + 1)| < 10<sup>-2</sup> 

(n + 1)/(2n + 1) < ε //*2n<sup>2</sup> - 1 
n + 1 < 2εn<sup>2</sup> - n - (ε + 1) 
n<sub>1, 2</sub> = (1 +- sqrt(1 + 8ε(ε + 1))) / (4ε) 
n<sub>1</sub> = 24.5025(valami jel) = 24 = n<sub>ε</sub> 
n<sub>2</sub> = ⚡︎

#### ?
lim n → inf (sqrt(3n<sup>2</sup> + 2) + sqrt(2n))/(sqrt(n<sup>3</sup> + n + 16, 4) - 3n) = -sqrt(3)/3 

#### ?
lim n → inf sqrt(4n <sup>2</sup> + 5n - 7) - 2n = ((sqrt(4n <sup>2</sup> + 5n - 7) - 2n) * (sqrt(4n <sup>2</sup> + 5n - 7) " 2n))/(sqrt(4n <sup>2</sup> + 5n - 7) + 2n) 
= (4n <sup>2</sup> + 5n - 7 - 4n <sup>2</sup>)/(sqrt(4n <sup>2</sup> + 5n - 7) + 2n) = (5 - 7/n)/(sqrt(4 + 5/n - 7/n <sup>2</sup>) + 2) = 5/(sqrt(4) + 2) = 5/(2 + 2) = 5/4 

#### ?
lim n → inf n(sqrt(n <sup>4</sup> + 4) - n <sup>2</sup>) = lim n → inf (4/n)/(sqrt(1 + 4/n <sup>4</sup>) + 1) = 0 

#### ?
lim n → inf = sqrt(n + sqrt(n + sqrt(n))) - sqrt(n) = 1/2

**Szabály**: lim n → inf (1 + C/a <sub>n</sub>)<sup>a <sub>n</sub></sup> = e <sup>c</sup> 
e <sup>-1</sup> = 1/e

lim n → inf ((2n + 3)/(2n - 2)) <sup>n - 5</sup> = ((2n - 2 + 5)/(2n - 2)) <sup>n - 5</sup> = (1 + 5/(2n - 2)) <sup>n - 5</sup>