|a_ × b_| = |a_| * |b_| * sin(fí)

# 1.
**a)**  
|a_| = 4  
|b_| = 5  
fí = 30°

|a_ × b_| = |a_| * |b_| * sin(fí) = 4 * 5 * sin(30°)

**b)**  
|a_| = 2 
|b_| = 13  
fí = 45°

|a_ × b_| = 2 * 13 * sqrt(45°) = 2 * 13 * sqrt(2) / 2 = 13 * sqrt(2)

**c)**  
|a_| = 6 
|b_| = 4  
fí = 120°

|a_ × b_| = 2 * 13 * sqrt(2) / 2 = 13 * sqrt(2)

**d)**  
a_ = 13  
b_ = 11  
fí = 90°

|a_ × b_| = 13 * 11 * sin(90°) = 13 * 11 * 1 = 143

**e)**  
|a_| = 3  
|b_| = 7  
fí = 180°

|a_ × b_| = 4 * 7 * sin(180°) = 4 * 7 * 0 = 0

# 2.
**a)**  
(a_ + b_) × (a_ - 2 * b_) = (a_ × a_) + (a_ × (-2 * b_)) + (b_ × a_) + (b_ × (-2 * b_))  
= -2 * (a_ × b_) - (a_ × b_) = -3(a_ × b_)

**b)**  
(3 * a_ - b_) × (b_ + 3 * a_) = (3 * a_ × b_) + (3 * a_ × 3 * a_) + (-b_ × b_) + ( -b_ × 3 * a_)  
= 3 * (a_ × b) - 3 * (b_ × a_) = 3 * (a_ × b_) + 3 * (a_ × b_) = 6 * (a_ × b_)

**c)**  
(a_ + 2 * b_) × (2 * a_ + b_) = -3(a_ × b_)

# 3.
a_ = (2; -3; 1)  
b_ = (4; 2; -1)  
c_ = (1; 0; -3)  
v_ = (a_ × b_) × c_

a_ × b_ = |i_ j_ k_ 2 -3 1 4 2 -1| = i_ * ((-3) * (-1) - 1 * 2) - j_ * (2 * (-1) - 1 * 4) + k_ * (2 * 2 - (-3) * 4)  
= i_ * (3 - 2) - j_ * (-2 - 4) + k_ (4 + 12) = i_ + j_ * 6 + k_ * 16 = (1; 6; 16)

v_ = (a_ × b_) × c_ = (1; 6; 16) × (1; 0; -3) = |i_ j_ k_ 1 6 16 1 0 -3|  
= i_ * (6 * -3 - 0 * 16) - j_ * (1 * -3 - 1 * 16) + k_ * (1 * 0 - 1 * 6)  
= i_ * -18 - j_ * -19 + k_ * -6 = (-18; 19; -6)

# 4.
a_ = (2; -3; 1)  
b_ = (1; -2; 3)  
c_ = (1; 2; -7)

c_ * x_ = 10
x_ _|_ a_
a_ _|_ b_

x_ || (a_ × b_) => x_ = lambda * (a_ × b_)  
a_ × b_ = (-7; -5; -1)
x_ = lambda * (a_ × b_) = lambda * (-7; -5; -1) = (-7 * lambda; -5 * lambda; -1 * lambda)

c_ * x_ = (1; 2; -7) * (-7 * lambda; -5 * lambda; -1 * lambda) = -7 * lambda - 10 * lambda + 7 * lambda = 10  
10 * lambda = 10  
lambda = 1

# 8.
a_ × b_ = t<sub>paralelogramma</sub>  
(2 * a_ + 3 * b_) × (4 * a_ - 2 * b_) = -4 * (a_ × b_) + 12 * (b_ × a_) = (-16) * (a_ × b_) = -16 * t<sub>paralelogramma</sub>

# 6.
A = (4, −1, −3)  
B = (3,  1, −2)  
C = (1,  5,  0)

AB_ = B - A = (-1; 2; 1)  
AC_ = C - A = (-3; 6; 3)

T<sub>paralelogramma</sub> = |AB_ × AC_|  
T<sub>háromszög</sub> = T<sub>paralelogramma</sub> / 2

-1 2 1
-3 6 3

AB_ × AC_ = |i_ j_ k_ -1 2 1 -3 6 3| = i_ * (2 * 3 - 6 * 1) - j_ * (-1 * 3 - (-3) * 1) + k_ * (-1 * 6 - (-3) * 2)  
= i_ * 0 - j_ * 0 + k_ * 0 = 0_

# 7.
A = (2,  3,  1)  
B = (4,  1, −2)  
C = (6,  3,  7)  
D = (−5, −4, 8)

ABC AC_ × AB_  
ACD AC_ × AD_

AB_ = (2;  -3; 4)  
AC_ = (4;   0; 6)  
AD_ = (-7; -7; 7)

AC_ × AB_ = (i_ j_ k_ 4 0 6 2 -2 3) = i_ * 12 - j_ * -24 + k_ * -8  
= (12; 24; -8) -> (3; 6; -2)

AC_ × AD_ = (3; -5; -2)

cos(fí) = ((3; 6; -2) * (3; -5; -2)) / (|(3; 6; -2)| * |(3; -5; -2)|) = 0,4  
fí = 113,2°  
180° - 113,2° = 66,8°