### 1.
#### a)
2(cos(30°) + i * sin(30°)) = 2(sqrt(3)/2 + i * 1/2) = sqrt(3) + i  

#### d)
3 * e<sup>n * i</sup> = 3(cos(pi) + i * sin(pi)) = 3(-1 + i * 0) = -3  

### 2.
#### a)
3 + 7i = sqrt(58) * (cos(66,8°) + i * sin(66,8°)) = sqrt(58) * e<sup>66,8° * pi/180</sup>  
r = |z| = sqrt(9 + 49) = sqrt(58)  
tan(fí) = b/a -> fí = arctan(b/a) = 66,8° = 66,8° * pi/180  

#### b)
-8 + 5i = sqrt(89) * (cos(148°) + i * sin(148°)) = sqrt(89) * e<sup>i * 37/45 * pi</sup>  
r = |z| = sqrt(64 + 25) = sqrt(89)  
fí = arctan(5/(-8)) = -32° + 180° = 148°  

### 4.
#### a)
(cos(pi/4) + i * sin(pi/4)) * (cos(3pi/4) + i * sin(3pi/4)) = cos(pi) + sin(pi) = e<sup>i * pi</sup> = -1  

#### b)
(cos(pi/3) + i * sin(pi/3))/(cos(5pi/6) + i * sin(5pi/6)) = cos(-3/6 * pi) + i * sin(-3/6 * pi) = cos(-pi/2) + i * sin(-pi/2) = e<sup>-pi/2 * i</sup> = -1  

#### d)
(cos(5pi/12) + i * sin(5pi/12))<sup>2</sup> = cos(5pi/6) + i * sin(5pi/6)  

### 6.
#### a)
z<sup>3</sup> = 27 * (cos(150°) + i * sin(150°))  
z = sqrt(27 * (cos(150°) + i * sin(150°)), 3)  
z = 3 * (cos(150°/3 + (k * 360°)/3) + i * sin(150°/3 + (k * 360°)/3)) = 3 * (cos(50° + k * 120°) + i * sin(50° + k * 120°))  
k eleme {0, 1, 2}  

z<sub>1</sub> = 3 * (cos(50° ) + i * sin(50° ))  
z<sub>2</sub> = 3 * (cos(170°) + i * sin(170°))  
z<sub>3</sub> = 3 * (cos(290°) + i * sin(290°))  

#### b)
z<sup>5</sup> = -32  
z<sup>5</sup> = -32 + i * 0 = 32 * (cos(180°) + i * sin(180°))  
z = sqrt(32 * (cos(180°) + i * sin(180°)), 5)  
z = 2 * (cos(180°/5 + k * 360°/5) + i * sin(180°/5 + k * 360°/5))  
z = 2 * (cos(36° + k * 72°) + i * sin(36° + k * 72°))  

z<sub>1</sub> = 2 * (cos( 36°) + i * sin( 36°))  
z<sub>2</sub> = 2 * (cos(108°) + i * sin(108°))  
z<sub>3</sub> = 2 * (cos(180°) + i * sin(180°))  
z<sub>4</sub> = 2 * (cos(252°) + i * sin(252°))  
z<sub>5</sub> = 2 * (cos(325°) + i * sin(325°))  
k eleme (0, 1, 2, 3, 4)  

### 7.
Írja fel a 6. egységgyökét  
sqrt(1, 6) = sqrt(cos(0°) + i * sin(0°), 6)  
1 = cos(0°/6 + k * 360°/6) + i * sin(0°/6 + k * 360°/6)  
1 = cos(0° + k * 60°) + i * sin(0° + k * 60°)  

### 8.
#### a)
z<sub>1</sub> = 3 * (cos(75°) + i * sin(75°)) = 3 * (cos(255°) + i * sin(255°))  

#### b)
z<sub>2</sub> = 6 * (cos(132°) - i * sin(132°))  
z<sub>2</sub> = 6 * (cos(-132°) + i * sin(-132°))  
z<sub>2</sub> = 6 * (cos(228°) + i * sin(228°))  

#### c)
z<sub>3</sub> = 24 * (cos(260°) - i * sin(260°))  
z<sub>3</sub> = 24 * (cos(180°) + i * sin(180°)) * (cos(-260°) + i * sin(-260°))  
z<sub>3</sub> = 24 * (cos(180°) + i * sin(180°)) * (cos(100°) + i * sin(100°))  
z<sub>3</sub> = 24 * (cos(280°) + i * sin(280°))  
