#### 1. d)
(6x - 2y)(6x + 2y) = 36x<sup>2</sup> - 4y<sup>2</sup>  

#### 2. c)
12x<sup>2</sup> + 12xy + 3y<sup>2</sup> = (sqrt(12)x + sqrt(3)y)<sup>2</sup>  
a<sup>4</sup> * a<sup>11</sup> = a<sup>15</sup>  

### 2.
#### c)
(2p<sup>4</sup>/q - p<sup>3</sup>/q<sup>2</sup>) * (2p4/q + p<sup>3</sup>/p<sup>2</sup>) = 4p<sup>8</sup>/q<sup>2</sup> - p<sup>6</sup>/q<sup>4</sup>  
#### d)
(1 + 2p + 4p<sup>2</sup>) * (2q + 3pq - p<sup>2</sup>q) = q(1 + 2p + 4p<sup>2</sup>)(2 + 3p - p<sup>2</sup>)  
= -4p<sup>4</sup> + 10p<sup>3</sup>q + 13p<sup>2</sup>q + 7pq + 2q  

#### 1. a)
sqrt(5) + sqrt(20) = sqrt(5) + sqrt(4 * 5) = sqrt(5) + 2 * sqrt(5) = 3 * sqrt(5)  

### 4.
#### a)
sqrt(27x<sup>6</sup>, 3) = sqrt(3<sup>3</sup>(x<sup>2</sup>)<sup>3</sup>, 3) = 3x<sup>2</sup>  

#### c)
(sqrt(2a + b) * sqrt(6bc))/(sqrt(15ac) * sqrt(5b<sup>4</sup>)) = sqrt(12ab<sup>2</sup>c/75ab<sup>2</sup>c) = 2/56  

#### 2. a)
(x<sup>0.5</sup> + y<sup>0.5</sup>)<sup>2</sup> = (x<sup>0.5</sup>)<sup>2</sup> + 2x<sup>0.5</sup> + y<sup>0.5</sup> + (y<sup>0.5</sup>)<sup>2</sup> = x + 2 * sqrt(x) * sqrt(y) + y  

#### 4. d)
sqrt(sqrt(3x<sup>7</sup>, 4), 3) = sqrt(3x<sup>7</sup>, 12) = 3<sup>1/12</sup>x<sup>7/12</sup>  

#### 1. g)
(2<sup>n</sup> + 3<sup>m</sup>)<sup>2</sup> = (2<sup>n</sup>)<sup>2</sup> + 2 * 2<sup>n</sup> + (3<sup>m</sup>)<sup>2</sup> = 2<sup>2n</sup> + 2<sup>n + 1</sup> * 3<sup>m</sup> + 3<sup>2m</sup>  

#### 3. c)
4x<sup>3</sup>y - 8xy<sup>3</sup> = 4xy(x<sup>2</sup> - 2y<sup>2</sup>)

#### 4. a)
sqrt(x<sup>2</sup>, 3) - sqrt(y<sup>2</sup>, 3) = x<sup>2/3</sup> - y<sup>2/3</sup> = (x<sup>2/3</sup>)<sup>2</sup> - (y<sup>2/3</sup>)<sup>2</sup>

#### 5. c)
4<sup>n</sup> + 9<sup>n</sup> + 2 * 6<sup>n</sup> = (2<sup>2</sup>)<sup>n</sup> + (3<sup>2</sup>)<sup>n</sup> + 2(2 * 3)<sup>n</sup> = (2<sup>n</sup>)<sup>2</sup> + (2<sup>n</sup>)<sup>2</sup> + 2 * 2<sup>n</sup> * 3<sup>n</sup> = (2<sup>n</sup> + 3<sup>n</sup>)<sup>2</sup>

### 1.
#### a)
(4x<sup>2</sup> - 15x + 9)/(x - 3) = 9  
((x - 3)(4x - 3))/(x - 3) = 9  
4x - 3 = 9  
4x = 12  
x = 3 ⚡︎ nincs megoldása

#### b)
(5x<sup>2</sup> - 28x + 23)/(x - 1) = -3  
5x<sup>2</sup> - 28x + 23 = -3x + 3  
5x<sup>2</sup> - 25x + 20 = 0  
x<sub>1</sub> = 4  
x<sub>2</sub> = 1

#### c)
(2x - 1)(x - 8) = 5(x - 8)  
2x - 1 = 5

#### d)
(x - 1)(x - 2)(x - 3) = 2(x - 3)  
(x - 1)(x - 2) = 2  
x<sup>2</sup> - 3x + 2 = 2  
x<sup>2</sup> - 3x = 0  
x<sub>1</sub> = 0  
x<sub>2</sub> = 3

### 4.
#### a)
4x - 3 >= x + 21  
3x - 24 >= 0  
3(x - 8) >= 0  
y - 8 >= 0  
x >= 8x

#### b)
(2x - 12)/(x + 2) > 0  
2x - 12 > 0 és x + 2 > 0  
vagy  
2x - 12 < 0 és x + 2 < 0  
x > 6 és x > -2  
vagy  
x < 6 és x < -2  

(3x - 4)/(2x + 1) >= 1  
(3x - 4)/(2x + 1) - 1 >= 0  
(3x - 4)/(2x + 1) - (2x + 1)/(2x + 1) >= 0  
(x - 5)/(2x + 1) >= 0