# Egyenesek
## 1.
P<sub>0</sub> = (-2, 3)  
#### a)
v_ = (4, 7)  

n_ normálvektor
n_ * v_ = 0  
n<sub>1</sub> * 4 + n<sub>2</sub> * 7 = 0  
n<sub>1</sub> * 4 = -n<sub>2</sub> * 7  
n_(-7, 4)  

#### b)
m = v<sub>2</sub>/v<sub>1</sub> = 7/4  

#### c)
v<sub>2</sub> * x - v<sub>1</sub> * y = v<sub>2</sub> * x<sub>0</sub> - v<sub>1</sub> * y<sub>0</sub>  
7x - 4y = -7(-2) - 4 * 3  
7x - 4y = -26  
-4y = -7x - 26  
y = (7/4)x + 26/4 = (7/4)x + 13/2

#### d)
A = (6, u)  
7 * 6 - 4u = -26  
4u = -68  
u = 17

## 2.
P(-2, 4)  
Q(6, 10)

#### a)
v_ = Q - P = (6, 10) - (-2, 4) = (8, 6)

#### b)
n_ * v_ = 0  
n<sub>1</sub> * 8 + n<sub>2</sub> * 6 = 0  
n<sub>1</sub> * 8 = -n<sub>2</sub> * 6  
n_(-6, 8)

#### c)
m = v_<sub>2</sub> / v_<sub>1</sub> = 6/8 = 3/4

#### d)
6x - 8y = -12 - 32  
-8y = -6x - 44  
8y = 6x + 44  
y = 3/4x + 11/4

#### e)
x = x<sub>0</sub> + t * v<sub>1</sub>  
y = y<sub>0</sub> + t * v<sub>2</sub>  
t eleme R  

x = -2 + 8t  
y = 4 + 6t

## 4.
P(4, 5)  
2x − 3y = 10

v_ = (3, 2)  
2x − 3y = 2 * 4 - 3 * 5  
2x − 3y = -7

## 8.
3x − 2y = 30  
x + 4y = −32  

(*2)  
6x - 4y = 60  
x + 4y = -32  
7x = 28  
x = 4

12 - 2y = 30  
-2y = 18  
y = -9

M(4, -9)

## 9.
P(10, 4)  
2x + 3y = 6

v_(-3, 2)  
n_(A, B)

Ax + By = Ax<sub>0</sub> + By<sub>0</sub>  
-3x + 2y = -3 * 10 + 2 * 4  
-3x + 2y = -22

# Tér
## 1.
P<sub>0</sub>(−2, 1, 4)  
v_(3, 2, −4)

#### a)
x = -2 + 3t  
y = 1 + 2t  
z = 4 - 4t  
t eleme R

#### b)
(x - x<sub>0</sub>)/v_<sub>1</sub> = (y - y<sub>0</sub>)/v<sub>2</sub> = (z - z<sub>0</sub>)/v<sub>3</sub>  
(x + 2)/3 = (4 - 2)/2 = (2 - 4)/(-4)

#### c)
P(34, 26, −44)  
34 = -2 + 3t  
26 = 1 + 2t  
-44 = 4 - 4t  

nincs rajta mert

## 3.
P<sub>0</sub>(-4, 2, -5)  
n_(2, 7, -2)

itt volt valami

## 4.
−x + 3y + 2z = 17  
n_(-1, 3, 2)

-1 + 6 + 2z = 17  
2t = 12  
z = 6

P(1, 2, 6)

## 6.
A(1, 3, -1)  
B(3, 1, 2)  
C(-6, 1, -3)

n_ = AB_ * AC_ = (2, -2, 3) * (-7, -2, -2) =
|i_ j_ k_|
| 2 -2  3|
|-7 -2 -2| = ((-2) * (-2) - (-2) * 3) - (2 * (-2) - (-7) * 3) + (2 * (-2) - (-7) * (-2)) = (4 - (-6)) - (-4 - (-21)) + (-4 - 14) = (10, -17, 18)  
AB_ = (3, 1, 2) - (1, 3, -1) = (2, -2, 3)  
AC_ = (-6, 1, -3) - (1, 3, -1) = (-7, -2, -2)

10(x - 9) - 17(y - 3) - 18(z + 4) = 0  
10x - 17y - 18z = -13

## 7.
x = -3 + 2t  
y = 2 + t  
z = 6 - 2t

2x − y − 2z = 15  
2(-3 + 2t) - (2 + t) - 2(6 - 2t) = 15  
-6 + 4t - 2 - t - 12 + 4t = 15  
-20 + 7t = 15  
7t = 35  
t = 5

x = -3 + 2 * 5 = 7  
y = 2 + t = 7  
z = 6 - 2 * 5 = -4  
P(7, 7, -4)

## 9.
P(1, 3, 2)  
−2x + y + 3z = 1  
x − y − z + 2 = 0

n<sub>1</sub> = (-2, 1, 3)  
n<sub>2</sub> = (1, -1, -1)

v_ = n<sub>1</sub> * n<sub>2</sub> = (2, 1, 1)  

P, v_
x = 1 + 2t  
y = 3 + t  
z = 2 + t