sin(Alpha + Beta) = sin(Alpha) * cos(Beta) + cos(Alpha) * sin(Beta)  
cos(Alpha + Beta) = cos(Alpha) * cos(Beta) + sin(Alpha) * sin(Beta)  
sin(2Alpha) = 2 * sin(Alpha) * cos(Alpha) * cos(Alpha) = cos<sup>2</sup>(Alpha) - sin<sup>2</sup>(Alpha)  
sin(Alpha - Beta) = sin(Alpha) * cos(Beta) - cos(Alpha) * sin(Beta)  
cos(Alpha - Beta) = cos(Alpha) * cos(Beta) - sin(Alpha) * sin(Beta)  
sin<sup>2</sup>(Alpha) = (1 - cos(2Alpha)) / 2  
sin<sup>2</sup>(Alpha) = (1 - cos(2Alpha)) / 2  
tan(Alpha + Beta) = (tan(Alpha) + tan(Beta)) / (1 - tan(Alpha) * tan(Beta))  
tan(Alpha - Beta) = (tan(Alpha) - tan(Beta)) / (1 + tan(Alpha) * tan(Beta))  
tan(2Alpha) = (2 * tan(Alpha)) / (1 - tan<sup>2</sup>(Alpha))  
sin<sup>2</sup>(Alpha) + cos<sup>2</sup>(Alpha) = 1  
tan(Alpha) = sin(Alpha) / cos(Alpha)  
ctg(Alpha) = cos(Alpha) / sin(Alpha)

sin(30°) = 1/2  
cos(30°) = sqrt(2) / 2  
tan(30°) = 1 / sqrt(2)  
ctg(30°) = sqrt(3)  

sin(45°) = 1 / sqrt(2)  
cos(45°) = 1 / sqrt(2)  
tan(45°) = 1  
ctg(45°) = 1  

sin(60°) = sqrt(3) / 2  
cos(60°) = 1/2  
tan(60°) = sqrt(3)  
ctg(60°) = 1 / sqrt(3)  

sin(90°) = 1  
cos(90°) = 0  
tan(90°) =   
ctg(90°) =   

sin(120°) = sqrt(3) / 2  
cos(120°) = 1 / 2  
tan(120°) =   
ctg(120°) =  

#### 1.
**a)**  
sin(2Alpha + Beta) = sin(2Alpha) * cos(Beta) + cos(2Alpha) * sin(Beta)  
2 * sin(Alpha) * cos(Alpha) * cos(Beta) + (cos<sup>2</sup>(Alpha) - sin<sup>2</sup>(Alpha)) * sin(Beta)

**f)**  
sin(3Alpha) = sin(2Alpha + Alpha) = sin(2Alpha) * cos(Alpha) + cos(2Alpha) * sin(Alpha)  
2 * sin(Alpha) * cos(Alpha) * cos(Alpha) + (cos<sup>2</sup>(Alpha) - sin<sup>2</sup>(Alpha)) * sin(Alpha)  
2 * sin(Alpha) * cos<sup>2</sup>(Alpha) + sin(Alpha) * cos<sup>2</sup>(Alpha) - sin<sup>2</sup>(Alpha) = 3 * sin(Alpha) * cos<sup>2</sup>(Alpha) - sin<sup>2</sup>(Alpha)

#### 2.
**b)**  
sin(x + 45°) = sin(x) * cos(45°) + cos(x) * sin(45°)  
(1 / sqrt(2)) * sin(x) + (1 / sqrt(2)) * cos(x)

**d)**  
sin(2y + 60°) = sin(2y) * cos(60°) + cos(2y) * sin(60°)  
(2 / 2) * sin(y) * cos(y) + (sqrt(3) / 2) * cos<sup>2</sup>(y) - (sqrt(3) / 2) * sin<sup>2</sup>(y)

#### 3.
**a)**  
(sin(Alpha) + cos(Alpha))<sup>2</sup> = 1 + sin(2Alpha)  
1 + sin(2Alpha)

**c)**  
(tan(Alpha) + 1)<sup>2</sup> = (1 + sin(2Alpha)) / cos<sup>2</sup>(Alpha)  
tan<sup>2</sup>(Alpha) + 2 * tan(Alpha) + 1 = sin<sup>2</sup>(Alpha) / cos(Alpha) + (2 * sin(Alpha)) / cos(Alpha) + cos<sup>2</sup>(Alpha) / cos<sup>2</sup>(Alpha) - sin<sup>2</sup>(Alpha) / sin<sup>2</sup>(Alpha) + (2 * sin(Alpha) * cos(Alpha)) / cos<sup>2</sup>(Alpha) + cos<sup>2</sup>(Alpha) / cos<sup>2</sup>(Alpha)  
(sin<sup>2</sup>(Alpha) + cos<sup>2</sup>(Alpha) + 2 * sin(Alpha) * cos(Alpha)) / cos<sup>2</sup>(Alpha) = (1 + sin(2Alpha)) / cos<sup>2</sup>(Alpha)

**h)**  
sin(x + 45°) * cos(x + 45°) = (cos <sup>2</sup>(x) - sin <sup>2</sup>(x)) / 2  
(sin(x) * cos(45°) + cos(x) * sin(45°)) * (cos(x) * cos(45°) - sin(x) * sin(45°)) = ((sqrt(2) / 2) * sin(x) + (sqrt(2) / 2) * cos(x))((sqrt(2) / 2) * cos(x) - (sqrt(2) / 2) * sin(x)) = ezt már nem írtam le

#### 4.
**c)**  
sin <sup>4</sup>(x) = (sin <sup>2</sup>(x))<sup>2</sup> = (1 - cos(2x)) <sup>2</sup> / 4 = 1/4 * (1 - 2 * cos(2x) + cos <sup>2</sup>(2x)) = 1/4 * (1 - 2 * cos(2x) + (1 + cos(4x)) / 2) = 1/4 - 1/2 * cos(2x) + 1/8 + 1/8 * cos(4x)

**d)**  
cos <sup>4</sup>(x) = 