# Trigonometria
**1.**  
a = 4  
b = 3  
c = sqrt(3<sup>2</sup> + 4<sup>2</sup>) = 5

sin(Alpha) = 3/5  
cos(Alpga) = 4/5  
tan(Alpha) = 3/4
ctg(Alpha) = 4/3

**2.**  
a = 6  
c = 3  
b = sqrt(2<sup>2</sup> + b<sup>2</sup>) -> 36 = 4 + b<sup>2</sup>  
b<sup>2</sup> = 32 (innel olvashatatlon volt) = 4 * sqrt(2)

sin(Alpha) = 1/5
cos(Alpha) = 
tan(Alpha) =
ctg(Alpha) =

**3.**  
Alpha = 28,2°  
fí = 180° - 90° - 28,2°= 61,8°  
sin(Alpha) = a/5 -> a = 5 * sin(28,2°) = 2,36  
cos(Alpha) = b/5 -> b = 5 * cos(28,2°) = 4,41

**4.**  
c  
40cm  
210cm

Alpha = tan<sup>-1</sup>(210/40) = 79,22°  
Beta = tan<sup>-1</sup>(40/210) = 10,78°

c = sqrt(210<sup>2</sup> + 40<sup>2</sup>) = sqrt(45700)

**5.**  
a = 360cm  
Beesési szög = 20°

Alpha = 90° - 20°= 70°  
tan(a) = b/360 -> b = 360 * tan(70°) = 989,09cm

**6.**  
R = 5cm  
a = ?  
r = ?

sin(54°) = r/R -> r * 5 * sin(54°) = 4,045cm  
cos(54°) = (a/2)/R -> a = 2 * 5 * cos(54°) = 5,8785cm

**7.**  
m = 5,7 * sin(63,4°) = 5,097  
a = 5,7 * cos(63,4°) = 2,55  
b = 8,2 - a = 5,65  
c = sqrt(b<sup>2</sup> + m<sup>2</sup>) = 7,607

fí = 42,05  
gamma = 180° - 63,4° - fí = 74,55

**8.**  
fÍ = 3/5  
sin <sup>-1</sup>(3/5) = 36,87°  
cos(fí) = 0,79  
tan(fí) = 0,75  
ctg(fí) = 1,3

**9.** - függvények ábrázolása, inkább nem rajzoltam  

**10.**  
**a)**  
sin(x) = 1  
x <sub>1</sub> = Pi/2 + 2 * k * Pi  
x <sub>2</sub> = -Pi/2 + 2 * k * Pi  
k eleme R

**b)**  
sin(x) = -1  
x = -Pi/2 + 2 * k * Pi

**c)**  
sin(x) = 0  
x = k * Pi

**d)**  
sin(x) = 1/2  
x <sub>1</sub> = Pi/6 + 2 * k * Pi  
x <sub>2</sub> = 5Pi/6 + 2 * k * Pi

**12.**  
**f)**  
sin(x) = 1 + sin(-x)  
sin(x) = 1 - sin(x)    
2 * sin(x) = 1  
sin(x) = 1/2

x <sub>1</sub> = Pi/6 + 2 * k * Pi   
x <sub>2</sub> = 5Pi/6 + 2 * k * Pi

**g)**  
cos(x) = 1 + cos(-x)
0 = 1 ⚡︎

**13.**  
**a)**  
sin <sup>2</sup>(x) - 3 * sin(x) + cos <sup>2</sup>(x) = 0  
**(sin <sup>2</sup>(x) + cos <sup>2</sup>(x) = 1)**  
-3 * sin(x) + 1 = 0  
-sin(x) = 1/3

**b)**  
6 * sin <sup>2</sup>(x) - 5 * sin(x) + 1 = 0  
(2 * sin(x) - 1)(3 * sin(x) - 1) = 0  
2 * sin(x) - 1 -> sin(x) = 1/2  
3 * sin(x) - 1 -> sin(x) = 1/3

**14.**  
**a)**  
sin(2x) = sin(x)  
2 * sin(x) * cos(x) = sin(x)  
2 * sin(x) * cos(x) - sin(x) = 0  
sin(x) * (2 * cos(x) - 1) / 0  
sin(x) -> sin(x) = 0  
2 * cos(x) - 1 -> sin(x) = 1/2